IMP-_To_SAS+/IMP--_To_SAS++/IMP_Minus_Minus_To_SAS_Plus_Plus_Reduction.thy
@@ -3,36 +3,13 @@
 section "Reduction"
 
 theory IMP_Minus_Minus_To_SAS_Plus_Plus_Reduction 
-  imports IMP_Minus_Minus_To_SAS_Plus_Plus_State_Translations
+  imports IMP_Minus_Minus_To_SAS_Plus_Plus_State_Translations IMP_Minus_Minus_Subprograms
 begin
 
-definition domain :: "com \<Rightarrow> nat \<Rightarrow> domain_element list" where
-"domain c t = (let m = max 1 (max_constant c) in map (\<lambda>i. EV (Num i))  [0 ..<(t * m + 1)]) @ [EV \<omega>]"
+definition domain :: "domain_element list" where
+"domain = [EV Zero, EV One]"
 
-lemma zero_in_domain[simp]: "ListMem (EV (Num 0)) (domain c t)"
-  by (auto simp: domain_def Let_def ListMem_iff)
-
-lemma omega_in_domain[simp]: "ListMem (EV \<omega>) (domain c t)"
-  by (auto simp: domain_def Let_def ListMem_iff)
-
-lemma [simp]: "(EV \<omega>) \<in> set (domain c t)"
-  by (auto simp: domain_def Let_def ListMem_iff)
-
-lemma num_in_domain_iff[simp]: "EV (Num x) \<in> set (domain c t) = (x \<le> t * (max 1 (max_constant c)))"
-  by (auto simp: domain_def Let_def)
-
-lemma [simp]: "((PCV i) \<in> set (domain c t)) = False" 
-  by (auto simp: domain_def Let_def)
-
-lemma [simp]: "domain c t \<noteq> []"
-  by (simp add: domain_def)
-
-lemma [simp]: "y \<in> set (domain c t) \<Longrightarrow> EV (case y of EV y' \<Rightarrow> y') = y"
-  by (auto simp: domain_def Let_def)
-
-lemma [simp]: "EV y \<in> set (domain c t) 
-  \<longleftrightarrow> (case y of Num x \<Rightarrow> x \<le> t * (max 1 (max_constant c)) | \<omega> \<Rightarrow> True)"
-  by (cases y) (auto simp: domain_def Let_def)
+declare domain_def[simp]
 
 type_synonym operator = "(variable, domain_element) sas_plus_operator"
 type_synonym problem = "(variable, domain_element) sas_plus_problem"
@@ -40,77 +17,70 @@ type_synonym problem = "(variable, domain_element) sas_plus_problem"
 definition pc_to_com :: "(variable \<times> domain_element) list \<Rightarrow> com" where
 "pc_to_com l = (case  l ! 0 of (_, PCV x) \<Rightarrow> x)"
 
-fun com_to_operators :: "com \<Rightarrow> domain_element list \<Rightarrow> operator list" where
-"com_to_operators (SKIP) d = []" |
-"com_to_operators (v ::= aexp) d = 
-  (case aexp of
-    A a \<Rightarrow> (case a of
-      N val \<Rightarrow> [\<lparr> precondition_of = [(PC, PCV (v ::= aexp))], 
-                  effect_of = [(PC, PCV SKIP), (VN v, (if (EV (Num val)) \<in> set d then EV (Num val) else EV \<omega>))]\<rparr>] |
-      V var \<Rightarrow> map (\<lambda> x. \<lparr> precondition_of = [(PC, PCV (v ::= aexp)), (VN var, x)], 
-                           effect_of = [(PC, PCV SKIP), (VN v, x)]\<rparr>) d) |
-    Plus a b \<Rightarrow> map (\<lambda> x.  \<lparr> precondition_of = [(PC, PCV (v ::= aexp)), (VN a, x)], 
-                             effect_of = [(PC, PCV SKIP), (VN v, EV (case x of 
-      EV (Num y) \<Rightarrow> (if EV (Num (y + b)) \<in> set d then Num (y + b) else \<omega>) | 
-      _ \<Rightarrow> \<omega>))]\<rparr>) d | 
-    Sub a b \<Rightarrow> map (\<lambda> x. \<lparr> precondition_of = [(PC, PCV (v ::= aexp)), (VN a, x)], 
-                            effect_of = [(PC, PCV SKIP), (VN v, EV (case x of 
-      EV (Num y) \<Rightarrow> (if EV (Num (y - b)) \<in> set d then Num (y - b) else \<omega>) | 
-      _ \<Rightarrow> \<omega>))]\<rparr>) d)" |
-"com_to_operators (c1;; c2) d = 
+fun com_to_operators :: "com \<Rightarrow> operator list" where
+"com_to_operators (SKIP) = []" |
+"com_to_operators (v ::= b) = 
+   [\<lparr> precondition_of = [(PC, PCV (v ::= b))], 
+      effect_of = [(PC, PCV SKIP), (VN v, EV b)]\<rparr>]" |
+"com_to_operators (c1;; c2) = 
   (if c1 = SKIP then  [\<lparr> precondition_of = [(PC, PCV (c1 ;; c2))],
                                                    effect_of = [(PC, PCV c2)]\<rparr>]
-   else (let ops = com_to_operators c1 d in map (\<lambda> op. 
+   else (let ops = com_to_operators c1 in map (\<lambda> op. 
     (let c1' = pc_to_com (effect_of op) in 
       \<lparr> precondition_of = 
         list_update (precondition_of op) 0 (PC, PCV (c1 ;; c2)),
         effect_of = 
         list_update (effect_of op) 0 (PC, PCV (c1' ;; c2))\<rparr>)) ops))" |
-"com_to_operators (IF v\<noteq>0 THEN c1 ELSE c2) d = (let i = PCV (IF v\<noteq>0 THEN c1 ELSE c2)
-   in map (\<lambda> x. 
-    \<lparr> precondition_of = [(PC, i), (VN v, x)], 
-      effect_of = [(PC, PCV (if x = EV (Num 0) then c2 else c1))]\<rparr>) d)" |
-"com_to_operators (WHILE v\<noteq>0 DO c) d = (let i = PCV (WHILE v\<noteq>0 DO c) ;
-  j = PCV (c ;; (WHILE v\<noteq>0 DO c)); k = PCV SKIP in map (\<lambda> x. 
-    \<lparr> precondition_of = [(PC, i), (VN v, x)], 
-      effect_of = [(PC, (if x = EV (Num 0) then k else j))]\<rparr>) d)"
+"com_to_operators (IF vs\<noteq>0 THEN c1 ELSE c2) = (let i = PCV (IF vs\<noteq>0 THEN c1 ELSE c2)
+   in  \<lparr> precondition_of = (PC, i) # map (\<lambda>v. (VN v, EV Zero)) (remdups vs), 
+        effect_of = [(PC, PCV c2)]\<rparr> 
+      # map (\<lambda> v. 
+      \<lparr> precondition_of = [(PC, i), (VN v, EV One)], 
+         effect_of = [(PC, PCV c1)]\<rparr>) vs)" |
+"com_to_operators (WHILE vs\<noteq>0 DO c) = (let i = PCV (WHILE vs\<noteq>0 DO c) ;
+  j = PCV (c ;; (WHILE vs\<noteq>0 DO c)); k = PCV SKIP in 
+    \<lparr> precondition_of = (PC, i) # map (\<lambda>v. (VN v, EV Zero)) (remdups vs), 
+        effect_of = [(PC, k)]\<rparr> 
+      # map (\<lambda> v. 
+      \<lparr> precondition_of = [(PC, i), (VN v, EV One)], 
+         effect_of = [(PC, j)]\<rparr>) vs)"
 
-lemma precondition_nonempty[simp]: "op \<in> set (com_to_operators c d) 
+lemma precondition_nonempty[simp]: "op \<in> set (com_to_operators c) 
   \<Longrightarrow> length (precondition_of op) > 0"
-  by (induction c d arbitrary: op rule: com_to_operators.induct)
-    (auto split: aexp.splits if_splits atomExp.splits)
+  by (induction c arbitrary: op rule: com_to_operators.induct)
+    (auto simp: Let_def split: if_splits)
 
-lemma effect_nonempty[simp]: "op \<in> set (com_to_operators c d) 
+lemma effect_nonempty[simp]: "op \<in> set (com_to_operators c) 
   \<Longrightarrow> length (effect_of op) > 0"
-  by (induction c d arbitrary: op rule: com_to_operators.induct)
-    (auto split: aexp.splits if_splits atomExp.splits)
+  by (induction c arbitrary: op rule: com_to_operators.induct)
+    (auto simp: Let_def split: if_splits)
 
-lemma PC_in_effect_precondition: "op \<in> set (com_to_operators c d) 
+lemma PC_in_effect_precondition: "op \<in> set (com_to_operators c) 
   \<Longrightarrow> (\<exists>y1 y2. (PC, PCV y1) = (precondition_of op) ! 0 \<and> (PC, PCV y2) = (effect_of op) ! 0)"
-proof(induction c d arbitrary: op rule: com_to_operators.induct)
+proof(induction c arbitrary: op rule: com_to_operators.induct)
   case (2 v aexp d)
-  then show ?case by (cases aexp) (auto simp: Let_def split: atomExp.splits)
+  then show ?case by (cases aexp) (auto simp: Let_def)
 next
   case (3 c1 c2 d)
   have "c1 = SKIP \<or> c1 \<noteq> SKIP" by simp
   then show ?case using 3 precondition_nonempty effect_nonempty by (auto split: if_splits)
-qed auto
+qed(auto simp: Let_def)
 
-lemma fst_of_effect[simp]: "op \<in> set (com_to_operators c d) 
+lemma fst_of_effect[simp]: "op \<in> set (com_to_operators c) 
   \<Longrightarrow> fst (effect_of op ! 0) = PC" 
   using PC_in_effect_precondition by (metis fst_conv)
 
-lemma fst_of_precondition[simp]: "op \<in> set (com_to_operators c d) 
+lemma fst_of_precondition[simp]: "op \<in> set (com_to_operators c) 
   \<Longrightarrow> fst (precondition_of op ! 0) = PC" 
   using PC_in_effect_precondition by (metis fst_conv)
 
 lemma com_to_operators_seq_registers:
-  assumes "c1 \<noteq> SKIP" and  "op \<in> set (com_to_operators (c1 ;; c2) d)" 
+  assumes "c1 \<noteq> SKIP" and  "op \<in> set (com_to_operators (c1 ;; c2))" 
     and "(VN x, y) \<in> set (precondition_of op) \<or> (VN x, y) \<in> set (effect_of op)"
-  shows "\<exists>op'. op' \<in> set (com_to_operators c1 d) 
+  shows "\<exists>op'. op' \<in> set (com_to_operators c1) 
           \<and> ((VN x, y) \<in> set (precondition_of op') \<or> (VN x, y) \<in> set (effect_of op'))"
 proof -
-  obtain op' where "op' \<in> set (com_to_operators c1 d) 
+  obtain op' where "op' \<in> set (com_to_operators c1) 
     \<and> op = (let c1' = pc_to_com (effect_of op') in 
       \<lparr> precondition_of = 
         list_update (precondition_of op') 0 (PC, PCV (c1 ;; c2)),
@@ -124,10 +94,10 @@ proof -
 qed
 
 lemma com_to_operators_registers_in_d: 
-  "op \<in> set (com_to_operators c d) 
-  \<Longrightarrow> ((VN x, y) \<in> set (precondition_of op) \<or> (VN x, y) \<in> set (effect_of op)) \<Longrightarrow> EV \<omega> \<in> set d 
-  \<Longrightarrow> y \<in> set d"
-proof (induction c d arbitrary: op rule: com_to_operators.induct)
+  "op \<in> set (com_to_operators c) 
+  \<Longrightarrow> ((VN x, y) \<in> set (precondition_of op) \<or> (VN x, y) \<in> set (effect_of op))  
+  \<Longrightarrow> (y = EV Zero \<or> y = EV One)"
+proof (induction c arbitrary: op rule: com_to_operators.induct)
   case (3 c1 c2 d)
   have "c1 = SKIP \<or> c1 \<noteq> SKIP" by simp
   then show ?case
@@ -138,59 +108,65 @@ proof (induction c d arbitrary: op rule: com_to_operators.induct)
     assume "c1 = SKIP" 
     then show ?thesis using 3 by auto
   qed
-qed (auto simp: Let_def split: aexp.splits atomExp.splits if_splits domain_element.splits EVal.splits)
+qed (auto simp: Let_def split: if_splits domain_element.splits)
 
 lemma update_preserve_distinct: "distinct (map fst l) \<Longrightarrow> fst (l ! 0) = x 
   \<Longrightarrow> distinct (map fst (l[0 := (x, y)]))"
   by (induction l) auto
 
-lemma com_to_operators_variables_distinct: 
-  "op \<in> set (com_to_operators c d) \<Longrightarrow> (l = precondition_of op \<or> l = effect_of op)
-  \<Longrightarrow> distinct (map fst l)"
-by (induction c d arbitrary: op l rule: com_to_operators.induct)
- (auto simp: Let_def update_preserve_distinct split: aexp.splits atomExp.splits if_splits)
+lemma map_fst_pair[simp]: "map (fst \<circ> (\<lambda>v. (VN v, EV Zero))) vs = map VN vs"
+  by (induction vs) auto
 
-lemma PC_of_precondition[simp]: "op \<in> set (com_to_operators c d) 
+lemma distinct_map_VN[simp]: "distinct (map VN vs) = distinct vs" 
+  by (induction vs) auto
+
+lemma com_to_operators_variables_distinct: 
+  "op \<in> set (com_to_operators c) \<Longrightarrow> (l = precondition_of op \<or> l = effect_of op)
+  \<Longrightarrow> distinct (map fst l)"
+by (induction c  arbitrary: op l rule: com_to_operators.induct)
+ (auto simp: Let_def update_preserve_distinct split: if_splits)
+
+lemma PC_of_precondition[simp]: "op \<in> set (com_to_operators c) 
   \<Longrightarrow> (PC, y) \<in> set (precondition_of op) \<longleftrightarrow> y = PCV c"
   using com_to_operators_variables_distinct PC_in_effect_precondition
   apply(cases c)
-      apply(auto simp: pc_to_com_def split: aexp.splits atomExp.splits if_splits)
+      apply(auto simp: pc_to_com_def Let_def split:  if_splits)
   by(metis eq_key_imp_eq_value fst_of_precondition precondition_nonempty 
       set_update_memI update_preserve_distinct)+
 
-lemma [simp]: "op \<in> set (com_to_operators c d) 
+lemma map_of_precondition_of_op_PC[simp]: "op \<in> set (com_to_operators c) 
   \<Longrightarrow> (map_of (precondition_of op)) PC = Some (PCV c)"
   using PC_of_precondition com_to_operators_variables_distinct by auto
 
-lemma [simp]: "op \<in> set (com_to_operators c d) 
+lemma pc_to_com_precondition_of_op_PC [simp]: "op \<in> set (com_to_operators c) 
   \<Longrightarrow> pc_to_com (precondition_of op) = c"
   using PC_of_precondition  
   by (metis PC_in_effect_precondition domain_element.simps nth_mem old.prod.case pc_to_com_def 
       precondition_nonempty)
 
-lemma pc_to_com_effect[simp]: "op \<in> set (com_to_operators c d) 
+lemma pc_to_com_effect[simp]: "op \<in> set (com_to_operators c) 
   \<Longrightarrow> (PC, y) \<in> set (effect_of op) \<longleftrightarrow> y = PCV (pc_to_com (effect_of op))"
   using com_to_operators_variables_distinct PC_in_effect_precondition 
   by (auto simp: pc_to_com_def)
    (metis domain_element.simps effect_nonempty eq_key_imp_eq_value nth_mem old.prod.case)+
 
-lemma PC_of_effect[simp]: "op \<in> set (com_to_operators c d) 
+lemma PC_of_effect[simp]: "op \<in> set (com_to_operators c) 
   \<Longrightarrow> map_of (effect_of op) PC = Some (PCV (pc_to_com (effect_of op)))"
   using com_to_operators_variables_distinct PC_in_effect_precondition 
   by (auto simp: pc_to_com_def)
 
 lemma com_to_operators_PC_is_subprogram: 
-  "op \<in> set (com_to_operators c d)
+  "op \<in> set (com_to_operators c)
   \<Longrightarrow>  (pc_to_com (precondition_of op) \<in> set (enumerate_subprograms c)
       \<and> pc_to_com (effect_of op) \<in> set (enumerate_subprograms c))"
-  apply (induction c d arbitrary: op rule: com_to_operators.induct)
+  apply (induction c arbitrary: op rule: com_to_operators.induct)
   using c_in_all_subprograms_c precondition_nonempty effect_nonempty
-      by (auto simp: Let_def pc_to_com_def split: if_splits aexp.splits atomExp.splits)
+      by (auto simp: Let_def pc_to_com_def split: if_splits )
 
-lemma com_to_operators_variables_in_enumerate_variables: "op \<in> set (com_to_operators c d)
+lemma com_to_operators_variables_in_enumerate_variables: "op \<in> set (com_to_operators c)
   \<Longrightarrow> ((VN x, y) \<in> set (precondition_of op) \<or> (VN x, y) \<in> set (effect_of op))
   \<Longrightarrow> x \<in> set (enumerate_variables c)"
-proof (induction c d arbitrary: op rule: com_to_operators.induct)
+proof (induction c arbitrary: op rule: com_to_operators.induct)
   case (3 c1 c2 d)
   have "c1 = SKIP \<or> c1 \<noteq> SKIP" by auto
   then show ?case
@@ -199,7 +175,7 @@ proof (induction c d arbitrary: op rule: com_to_operators.induct)
     then show ?thesis using 3 by auto
   next
     assume "c1 \<noteq> SKIP"
-    moreover then obtain op' where "op' \<in> set (com_to_operators c1 d) 
+    moreover then obtain op' where "op' \<in> set (com_to_operators c1) 
           \<and> ((VN x, y) \<in> set (precondition_of op') \<or> (VN x, y) \<in> set (effect_of op'))"
       using 3 com_to_operators_seq_registers by metis
     moreover have "c1 \<in> set (enumerate_subprograms (c1 ;; c2))" using c_in_all_subprograms_c by auto
@@ -208,32 +184,33 @@ proof (induction c d arbitrary: op rule: com_to_operators.induct)
       by simp
     ultimately show ?thesis using 3 by auto
   qed
-qed (auto simp: Let_def split: aexp.splits atomExp.splits if_splits)
+qed (auto simp: Let_def split: if_splits)
 
-lemma [simp]: "op \<in> set (com_to_operators c1 (domain c t)) \<Longrightarrow> (VN v, PCV c') \<notin> set (effect_of op)"
+lemma VN_PCV_not_in_effect[simp]: 
+  "op \<in> set (com_to_operators c1) \<Longrightarrow> (VN v, PCV c') \<notin> set (effect_of op)"
   apply(induction c1 arbitrary: op)
-      apply(auto split: aexp.splits atomExp.splits if_splits)
+      apply(auto simp: Let_def split: if_splits)
   by (metis (no_types, lifting) in_set_conv_nth length_list_update nth_list_update 
       nth_list_update_neq prod.inject variable.distinct(1))
 
-lemma in_set_effect: "op \<in> set (com_to_operators c1 (domain c t)) 
+lemma in_set_effect: "op \<in> set (com_to_operators c1) 
   \<Longrightarrow> (VN v, y) \<in> set (effect_of op)
   \<Longrightarrow> \<exists>y'. y = EV y'"
   apply(induction c1 arbitrary: op)
-      apply(auto simp: domain_def Let_def split: aexp.splits atomExp.splits if_splits)
+      apply(auto simp: Let_def split: if_splits)
   by (metis in_set_conv_nth length_list_update nth_list_update nth_list_update_neq 
       prod.inject variable.distinct)
 
-lemma in_set_precondition: "op \<in> set (com_to_operators c1 (domain c t)) 
+lemma in_set_precondition: "op \<in> set (com_to_operators c1) 
   \<Longrightarrow> (VN v, y) \<in> set (precondition_of op)
   \<Longrightarrow> \<exists>y'. y = EV y'"
   apply(induction c1 arbitrary: op)
-      apply(auto simp: domain_def Let_def split: aexp.splits atomExp.splits if_splits)
+      apply(auto simp: domain_def Let_def split: if_splits)
   by (metis in_set_conv_nth length_list_update nth_list_update nth_list_update_neq 
       prod.inject variable.distinct)
 
 lemma map_of_precondition_eq_Some[simp]: 
-  assumes "op \<in> set (com_to_operators c1 (domain c t))"
+  assumes "op \<in> set (com_to_operators c1)"
    "map_of (precondition_of op) (VN v) = Some y"
  shows "\<exists>y'. y = EV y'"
 proof -
@@ -241,11 +218,11 @@ proof -
   then show ?thesis using assms in_set_precondition by simp
 qed
 
-lemma "op \<in> set (com_to_operators c1 (domain c t)) 
+lemma "op \<in> set (com_to_operators c1) 
   \<Longrightarrow> (VN v, y) \<in> set (effect_of op) 
   \<Longrightarrow> \<exists>x. (VN v, EV x) \<in> set (effect_of op)"
   apply(induction c1 arbitrary: op)
-      apply(auto simp: domain_def Let_def split: aexp.splits atomExp.splits if_splits)
+      apply(auto simp: domain_def Let_def split: if_splits)
   by (metis (no_types, lifting) Pair_inject com_to_operators_variables_distinct effect_nonempty 
       fst_of_effect in_set_conv_nth length_list_update map_of_eq_Some_iff nth_list_update 
       update_preserve_distinct variable.distinct)
@@ -256,7 +233,7 @@ lemma not_in_set_then_map_of_eq_None:
   by auto
 
 lemma variables_in_effect[simp]: 
-  assumes "op \<in> set (com_to_operators c1 (domain c t))"
+  assumes "op \<in> set (com_to_operators c1)"
   shows "\<exists>x. (VN v, EV x) \<in> set (effect_of op) \<or> map_of (effect_of op) (VN v) = None"
 proof -
   have "(\<exists>y. (VN v, y) \<in> set (effect_of op)) \<or> \<not>((\<exists>y. (VN v, y) \<in> set (effect_of op)))" by auto
@@ -265,8 +242,8 @@ proof -
     using assms in_set_effect apply blast using not_in_set_then_map_of_eq_None by simp
 qed
   
-lemma [simp]: 
-  assumes "op \<in> set (com_to_operators c1 d)"
+lemma in_precondition_not_VN_then_PC[simp]: 
+  assumes "op \<in> set (com_to_operators c1)"
     "(a, b) \<in> set (precondition_of op)"
     "c1 \<in> set (enumerate_subprograms c)"
     "a \<notin> VN ` set (enumerate_variables c)" 
@@ -278,8 +255,8 @@ proof (cases a)
   then show ?thesis using VN com_to_operators_variables_in_enumerate_variables assms by blast
 qed auto
 
-lemma [simp]: 
-  assumes "op \<in> set (com_to_operators c1 d)"
+lemma in_effect_not_VN_then_PC[simp]: 
+  assumes "op \<in> set (com_to_operators c1)"
     "(a, b) \<in> set (effect_of op)"
     "c1 \<in> set (enumerate_subprograms c)"
     "a \<notin> VN ` set (enumerate_variables c)" 
@@ -291,45 +268,44 @@ proof (cases a)
   then show ?thesis using VN com_to_operators_variables_in_enumerate_variables assms by blast
 qed auto
 
-definition coms_to_operators :: "com list \<Rightarrow> domain_element list \<Rightarrow> operator list" where
-"coms_to_operators cs d = concat (map (\<lambda> c. com_to_operators c d) cs)"
-
+definition coms_to_operators :: "com list \<Rightarrow> operator list" where
+"coms_to_operators cs = concat (map com_to_operators cs)"
 
 definition imp_minus_minus_to_sas_plus :: 
-"com \<Rightarrow> (vname \<rightharpoonup> EVal) \<Rightarrow> (vname \<rightharpoonup> EVal) \<Rightarrow> nat \<Rightarrow> problem" where
-"imp_minus_minus_to_sas_plus c I G t = (let cs = enumerate_subprograms c ; 
-  d = domain c t in let
+"com \<Rightarrow> imp_state \<Rightarrow> imp_state \<Rightarrow> problem" where
+"imp_minus_minus_to_sas_plus c I G = (let cs = enumerate_subprograms c ; 
   initial_vs = I|`(set (enumerate_variables c)) ;
   goal_vs = G|`(set (enumerate_variables c)) ;
   pc_d = map (\<lambda> i. PCV i) cs in
     \<lparr> variables_of = PC # (map VN (enumerate_variables c)),
-      operators_of = coms_to_operators cs d, 
+      operators_of = coms_to_operators cs, 
       initial_of = imp_minus_state_to_sas_plus (c, initial_vs),
       goal_of = imp_minus_state_to_sas_plus (SKIP, goal_vs),
-      range_of = (map_of (map (\<lambda> v. (VN v, d)) (enumerate_variables c)))(PC \<mapsto> pc_d)\<rparr>)"
+      range_of = (map_of (map (\<lambda> v. (VN v, domain)) (enumerate_variables c)))(PC \<mapsto> pc_d)\<rparr>)"
 
 lemma range_defined: 
-  assumes "v \<in> set (variables_of (imp_minus_minus_to_sas_plus c I G t))" 
-  shows "(\<exists>y. range_of (imp_minus_minus_to_sas_plus c I G t) v = Some y)"
+  assumes "v \<in> set (variables_of (imp_minus_minus_to_sas_plus c I G))" 
+  shows "(\<exists>y. range_of (imp_minus_minus_to_sas_plus c I G) v = Some y)"
 proof(cases v)
   case (VN x)
-  then have "(VN x, domain c t) \<in> set (map (\<lambda> v. (VN v, domain c t)) (enumerate_variables c))" 
+  then have "(VN x, domain) \<in> set (map (\<lambda> v. (VN v, domain)) (enumerate_variables c))" 
     using assms by (auto simp: Let_def imp_minus_minus_to_sas_plus_def)    
   then show ?thesis using VN by (auto simp: Let_def imp_minus_minus_to_sas_plus_def weak_map_of_SomeI) 
 qed (auto simp: imp_minus_minus_to_sas_plus_def Let_def)
 
 lemma range_non_empty: 
-  assumes "v \<in> set (variables_of (imp_minus_minus_to_sas_plus c I G t))" 
-  shows "(\<exists>y. y \<in> range_of' (imp_minus_minus_to_sas_plus c I G t) v)"
+  assumes "v \<in> set (variables_of (imp_minus_minus_to_sas_plus c I G))" 
+  shows "(\<exists>y. y \<in> range_of' (imp_minus_minus_to_sas_plus c I G) v)"
 proof (cases v)
   case (VN x)
-  then have *: "(VN x, domain c t) \<in> set (map (\<lambda> v. (VN v, domain c t)) (enumerate_variables c))" 
+  then have *: "(VN x, domain) \<in> set (map (\<lambda> v. (VN v, domain)) (enumerate_variables c))" 
     using assms by (auto simp: Let_def imp_minus_minus_to_sas_plus_def)
-  then have "range_of (imp_minus_minus_to_sas_plus c I G t) v = Some (domain c t)" 
-    using VN by (simp add: Let_def imp_minus_minus_to_sas_plus_def) 
-       (smt Pair_inject * ex_map_conv map_of_SomeD weak_map_of_SomeI)
-  then show ?thesis using assms VN by (simp add: range_of'_def)
-     (meson ListMem_iff omega_in_domain)
+  then have "range_of (imp_minus_minus_to_sas_plus c I G) v = Some domain" 
+    using VN
+    apply - apply(frule weak_map_of_SomeI)
+    apply (simp add: Let_def imp_minus_minus_to_sas_plus_def)
+    using map_of_SomeD by force 
+  thus ?thesis by(auto simp: range_of'_def)
 next
   case PC
   then show ?thesis using SKIP_in_enumerate_subprograms
@@ -358,18 +334,19 @@ qed
 lemma [simp]: "PCV x \<in> PCV ` y \<longleftrightarrow> x \<in> y" by auto
 
 lemma operators_valid: 
-  assumes "cs = enumerate_subprograms c" and "c1 \<in> set cs" and "d = domain c t"
-         and  "op \<in> set (com_to_operators c1 d)"
-  shows "is_valid_operator_sas_plus (imp_minus_minus_to_sas_plus c I G t) op" 
+  assumes "cs = enumerate_subprograms c" and "c1 \<in> set cs"
+         and  "op \<in> set (com_to_operators c1)"
+  shows "is_valid_operator_sas_plus (imp_minus_minus_to_sas_plus c I G) op" 
 proof -                   
-  let ?\<Psi> = "imp_minus_minus_to_sas_plus c I G t"
+  let ?\<Psi> = "imp_minus_minus_to_sas_plus c I G"
   let ?pre = "precondition_of op" and ?eff = "effect_of op" and ?vs = "variables_of ?\<Psi>" 
       and ?D = "range_of ?\<Psi>" and ?pc_d = "map (\<lambda> i. PCV i) (enumerate_subprograms c)"
 
   have *: "list_all (\<lambda>(v, a). ListMem v ?vs) ?pre \<and> list_all (\<lambda>(v, a). ListMem v ?vs) ?eff"
     using assms by(auto simp: imp_minus_minus_to_sas_plus_def Let_def ListMem_iff list_all_def)
 
-  have "((VN x, a) \<in> set ?pre \<or> (VN x, a) \<in> set ?eff) \<Longrightarrow> ?D (VN x) = Some d \<and> a \<in> set d" for x a
+  have "((VN x, a) \<in> set ?pre \<or> (VN x, a) \<in> set ?eff) \<Longrightarrow> ?D (VN x) = Some domain 
+    \<and> a \<in> set domain" for x a
     using assms com_to_operators_registers_in_d com_to_operators_variables_in_enumerate_variables
         enumerate_subprograms_enumerate_variables 
     by (fastforce simp: imp_minus_minus_to_sas_plus_def Let_def)    
@@ -395,11 +372,9 @@ lemma not_in_enumerate_variables_not_PC_then[simp]:
   apply(cases v) by auto
 
 lemma imp_minus_minus_to_sas_plus_valid:
-  assumes "(\<forall>x y. I x = Some (Num y) \<longrightarrow> y \<le> t * (max 1 (max_constant c)))"
-  assumes "(\<forall>x y. G x = Some (Num y) \<longrightarrow> y \<le> t * (max 1 (max_constant c)))"
-  shows "is_valid_problem_sas_plus_plus (imp_minus_minus_to_sas_plus c I G t)"
+  "is_valid_problem_sas_plus_plus (imp_minus_minus_to_sas_plus c I G)"
 proof -
-  let ?\<Psi> = "imp_minus_minus_to_sas_plus c I G t"
+  let ?\<Psi> = "imp_minus_minus_to_sas_plus c I G"
   let ?ops = "operators_of ?\<Psi>"
       and ?vs = "variables_of ?\<Psi>"
       and ?I = "initial_of ?\<Psi>"
@@ -414,10 +389,10 @@ proof -
     and "?I v \<noteq> None \<longrightarrow> ListMem (the (?I v)) (the (?D v))"
     and "?G v \<noteq> None \<longrightarrow> ListMem (the (?G v)) (the (?D v))" for v
        apply(cases v)
-       using c_in_all_subprograms_c[where ?c = c] SKIP_in_enumerate_subprograms assms
+       using c_in_all_subprograms_c[where ?c = c] SKIP_in_enumerate_subprograms
        by (auto simp: imp_minus_minus_to_sas_plus_def Let_def coms_to_operators_def 
         imp_minus_state_to_sas_plus_def map_comp_def ListMem_iff image_def 
-        split: variable.splits option.splits EVal.splits)
+        split: variable.splits option.splits)
     ultimately show ?thesis
     by (auto simp: is_valid_problem_sas_plus_plus_def range_defined list_all_def)
 qed
